src/_output/ocaml/Space_Bitwise.ml
@@ -1,0 +1,56 @@
+open Prims
+let bit_and (a : Space_Types.cell) (b : Space_Types.cell) : Space_Types.cell=
+  FStar_UInt64.logand a b
+let bit_or (a : Space_Types.cell) (b : Space_Types.cell) : Space_Types.cell=
+  FStar_UInt64.logor a b
+let bit_xor (a : Space_Types.cell) (b : Space_Types.cell) : Space_Types.cell=
+  FStar_UInt64.logxor a b
+let bit_not (a : Space_Types.cell) : Space_Types.cell= FStar_UInt64.lognot a
+let shift_left (a : Space_Types.cell) (n : FStar_UInt32.t) :
+  Space_Types.cell= FStar_UInt64.shift_left a n
+let shift_right (a : Space_Types.cell) (n : FStar_UInt32.t) :
+  Space_Types.cell= FStar_UInt64.shift_right a n
+let stack_and (s : Space_Stack.stack) :
+  Space_Stack.stack FStar_Pervasives_Native.option=
+  match s with
+  | a::b::xs -> FStar_Pervasives_Native.Some ((bit_and b a) :: xs)
+  | uu___ -> FStar_Pervasives_Native.None
+let stack_or (s : Space_Stack.stack) :
+  Space_Stack.stack FStar_Pervasives_Native.option=
+  match s with
+  | a::b::xs -> FStar_Pervasives_Native.Some ((bit_or b a) :: xs)
+  | uu___ -> FStar_Pervasives_Native.None
+let stack_xor (s : Space_Stack.stack) :
+  Space_Stack.stack FStar_Pervasives_Native.option=
+  match s with
+  | a::b::xs -> FStar_Pervasives_Native.Some ((bit_xor b a) :: xs)
+  | uu___ -> FStar_Pervasives_Native.None
+let stack_not (s : Space_Stack.stack) :
+  Space_Stack.stack FStar_Pervasives_Native.option=
+  match s with
+  | a::xs -> FStar_Pervasives_Native.Some ((bit_not a) :: xs)
+  | uu___ -> FStar_Pervasives_Native.None
+let stack_shl (s : Space_Stack.stack) :
+  Space_Stack.stack FStar_Pervasives_Native.option=
+  match s with
+  | n_cell::a::xs ->
+      let n = FStar_UInt64.v n_cell in
+      let shift = if n >= (Prims.of_int (64)) then (Prims.of_int (63)) else n in
+      let n32 =
+        FStar_Int_Cast.uint64_to_uint32 (FStar_UInt64.uint_to_t shift) in
+      if (FStar_UInt32.v n32) < (Prims.of_int (64))
+      then FStar_Pervasives_Native.Some ((shift_left a n32) :: xs)
+      else FStar_Pervasives_Native.Some (Stdint.Uint64.zero :: xs)
+  | uu___ -> FStar_Pervasives_Native.None
+let stack_shr (s : Space_Stack.stack) :
+  Space_Stack.stack FStar_Pervasives_Native.option=
+  match s with
+  | n_cell::a::xs ->
+      let n = FStar_UInt64.v n_cell in
+      let shift = if n >= (Prims.of_int (64)) then (Prims.of_int (63)) else n in
+      let n32 =
+        FStar_Int_Cast.uint64_to_uint32 (FStar_UInt64.uint_to_t shift) in
+      if (FStar_UInt32.v n32) < (Prims.of_int (64))
+      then FStar_Pervasives_Native.Some ((shift_right a n32) :: xs)
+      else FStar_Pervasives_Native.Some (Stdint.Uint64.zero :: xs)
+  | uu___ -> FStar_Pervasives_Native.None
