src/_output/ocaml/Space_Types.ml
@@ -1,0 +1,14 @@
+open Prims
+type cell = FStar_UInt64.t
+type universe_id = Prims.nat
+type universe_name = Prims.string
+type discipline =
+  | Unrestricted 
+  | Affine 
+  | Linear 
+let uu___is_Unrestricted (projectee : discipline) : Prims.bool=
+  match projectee with | Unrestricted -> true | uu___ -> false
+let uu___is_Affine (projectee : discipline) : Prims.bool=
+  match projectee with | Affine -> true | uu___ -> false
+let uu___is_Linear (projectee : discipline) : Prims.bool=
+  match projectee with | Linear -> true | uu___ -> false
