src/Space.Instruction.fst
@@ -8,9 +8,9 @@ open Space.Types
 (** Instruction pointer *)
 type ip = UInt64.t
 
-(** Primitive operations *)
+(** Primitive operations - 80 primitives *)
 type prim_op =
-  (* Stack manipulation *)
+  (* Stack manipulation - 8 ops *)
   | PrimDup
   | PrimDrop
   | PrimSwap
@@ -19,7 +19,7 @@ type prim_op =
   | PrimNip
   | PrimTuck
   | PrimPick
-  (* Arithmetic *)
+  (* Arithmetic - 9 ops *)
   | PrimAdd
   | PrimSub
   | PrimMul
@@ -29,34 +29,86 @@ type prim_op =
   | PrimNeg
   | PrimMin
   | PrimMax
-  (* Bitwise *)
+  (* Bitwise - 6 ops *)
   | PrimAnd
   | PrimOr
   | PrimXor
   | PrimNot
   | PrimShl
   | PrimShr
-  (* Comparison *)
+  (* Comparison - 6 ops *)
   | PrimEq
   | PrimNeq
   | PrimLtU
   | PrimGtU
   | PrimLtS
   | PrimGtS
-  (* Memory - cell level *)
+  (* Memory - cell level - 3 ops *)
   | PrimFetch
   | PrimStore
   | PrimAlloc
-  (* Memory - byte level *)
+  (* Memory - byte level - 5 ops *)
   | PrimBytesAlloc
   | PrimBytesFetch
   | PrimBytesStore
   | PrimBytesLen
   | PrimBytesCopy
-  (* System *)
+  (* Borrowing - 8 ops *)
+  | PrimBorrowPointer
+  | PrimReturnPointer
+  | PrimDropPointer
+  | PrimFetchBorrowed
+  | PrimStoreBorrowed
+  | PrimFetchAndEnd
+  | PrimStoreAndEnd
+  | PrimOffsetBorrowed
+  (* Warp - 7 ops *)
+  | PrimWarpFetch
+  | PrimWarpStore
+  | PrimWarpAdvance
+  | PrimWarpFollow
+  | PrimWarpPosition
+  | PrimWarpRestore
+  | PrimWarpNull
+  (* Text - 11 ops *)
+  | PrimCreateText
+  | PrimTextByteLength
+  | PrimTextGraphemeCount
+  | PrimTextIsSimple
+  | PrimTextGraphemeAt
+  | PrimTextGraphemeFirst
+  | PrimTextGraphemeLast
+  | PrimTextSlice
+  | PrimTextConcat
+  | PrimTextEqual
+  | PrimTextCompare
+  (* Text warp - 5 ops *)
+  | PrimTextWarpHasGrapheme
+  | PrimTextWarpCurrentGrapheme
+  | PrimTextWarpNextGrapheme
+  | PrimTextWarpGraphemeIndex
+  | PrimTextWarpGotoGrapheme
+  (* Grapheme properties - 3 ops *)
+  | PrimGraphemeByteLength
+  | PrimGraphemeIsAscii
+  | PrimGraphemeCodePoints
+  (* Code point access - 2 ops *)
+  | PrimTextCodePointCount
+  | PrimTextCodePointAt
+  (* System - 4 ops *)
   | PrimEmit
   | PrimKey
+  | PrimEmitGrapheme
   | PrimHalt
+  (* Normalization - 4 ops *)
+  | PrimTextNormalizeNfc
+  | PrimTextNormalizeNfd
+  | PrimTextNormalizeNfkc
+  | PrimTextNormalizeNfkd
+  (* Case mapping - 3 ops *)
+  | PrimTextToUpper
+  | PrimTextToLower
+  | PrimTextToTitle
 
 (** Instructions *)
 type instruction =
@@ -72,32 +124,105 @@ type instruction =
   | IReleaseUniverse of universe_name (* Release affine universe *)
   | ITransferTo of universe_name      (* Transfer value to named universe *)
 
-(** Decode primitive from opcode *)
+(** Decode primitive from opcode - 80 primitives *)
 let decode_prim (op: UInt64.t) : option prim_op =
+  (* Stack manipulation: 0-7 *)
   if op = 0uL then Some PrimDup
   else if op = 1uL then Some PrimDrop
   else if op = 2uL then Some PrimSwap
   else if op = 3uL then Some PrimOver
   else if op = 4uL then Some PrimRot
+  else if op = 5uL then Some PrimNip
+  else if op = 6uL then Some PrimTuck
+  else if op = 7uL then Some PrimPick
+  (* Arithmetic: 10-18 *)
   else if op = 10uL then Some PrimAdd
   else if op = 11uL then Some PrimSub
   else if op = 12uL then Some PrimMul
   else if op = 13uL then Some PrimDivU
-  else if op = 14uL then Some PrimMod
+  else if op = 14uL then Some PrimDivS
+  else if op = 15uL then Some PrimMod
+  else if op = 16uL then Some PrimNeg
+  else if op = 17uL then Some PrimMin
+  else if op = 18uL then Some PrimMax
+  (* Bitwise: 20-25 *)
   else if op = 20uL then Some PrimAnd
   else if op = 21uL then Some PrimOr
   else if op = 22uL then Some PrimXor
   else if op = 23uL then Some PrimNot
   else if op = 24uL then Some PrimShl
   else if op = 25uL then Some PrimShr
+  (* Comparison: 30-35 *)
   else if op = 30uL then Some PrimEq
   else if op = 31uL then Some PrimNeq
   else if op = 32uL then Some PrimLtU
   else if op = 33uL then Some PrimGtU
+  else if op = 34uL then Some PrimLtS
+  else if op = 35uL then Some PrimGtS
+  (* Memory cell: 40-42 *)
   else if op = 40uL then Some PrimFetch
   else if op = 41uL then Some PrimStore
   else if op = 42uL then Some PrimAlloc
-  else if op = 50uL then Some PrimEmit
-  else if op = 51uL then Some PrimKey
-  else if op = 52uL then Some PrimHalt
+  (* Memory bytes: 43-47 *)
+  else if op = 43uL then Some PrimBytesAlloc
+  else if op = 44uL then Some PrimBytesFetch
+  else if op = 45uL then Some PrimBytesStore
+  else if op = 46uL then Some PrimBytesLen
+  else if op = 47uL then Some PrimBytesCopy
+  (* Borrowing: 50-57 *)
+  else if op = 50uL then Some PrimBorrowPointer
+  else if op = 51uL then Some PrimReturnPointer
+  else if op = 52uL then Some PrimDropPointer
+  else if op = 53uL then Some PrimFetchBorrowed
+  else if op = 54uL then Some PrimStoreBorrowed
+  else if op = 55uL then Some PrimFetchAndEnd
+  else if op = 56uL then Some PrimStoreAndEnd
+  else if op = 57uL then Some PrimOffsetBorrowed
+  (* Warp: 60-66 *)
+  else if op = 60uL then Some PrimWarpFetch
+  else if op = 61uL then Some PrimWarpStore
+  else if op = 62uL then Some PrimWarpAdvance
+  else if op = 63uL then Some PrimWarpFollow
+  else if op = 64uL then Some PrimWarpPosition
+  else if op = 65uL then Some PrimWarpRestore
+  else if op = 66uL then Some PrimWarpNull
+  (* Text: 70-80 *)
+  else if op = 70uL then Some PrimCreateText
+  else if op = 71uL then Some PrimTextByteLength
+  else if op = 72uL then Some PrimTextGraphemeCount
+  else if op = 73uL then Some PrimTextIsSimple
+  else if op = 74uL then Some PrimTextGraphemeAt
+  else if op = 75uL then Some PrimTextGraphemeFirst
+  else if op = 76uL then Some PrimTextGraphemeLast
+  else if op = 77uL then Some PrimTextSlice
+  else if op = 78uL then Some PrimTextConcat
+  else if op = 79uL then Some PrimTextEqual
+  else if op = 80uL then Some PrimTextCompare
+  (* Text warp: 81-85 *)
+  else if op = 81uL then Some PrimTextWarpHasGrapheme
+  else if op = 82uL then Some PrimTextWarpCurrentGrapheme
+  else if op = 83uL then Some PrimTextWarpNextGrapheme
+  else if op = 84uL then Some PrimTextWarpGraphemeIndex
+  else if op = 85uL then Some PrimTextWarpGotoGrapheme
+  (* Grapheme: 86-88 *)
+  else if op = 86uL then Some PrimGraphemeByteLength
+  else if op = 87uL then Some PrimGraphemeIsAscii
+  else if op = 88uL then Some PrimGraphemeCodePoints
+  (* Codepoint: 89-90 *)
+  else if op = 89uL then Some PrimTextCodePointCount
+  else if op = 90uL then Some PrimTextCodePointAt
+  (* I/O: 100-103 *)
+  else if op = 100uL then Some PrimEmit
+  else if op = 101uL then Some PrimKey
+  else if op = 102uL then Some PrimEmitGrapheme
+  else if op = 103uL then Some PrimHalt
+  (* Normalization: 120-123 *)
+  else if op = 120uL then Some PrimTextNormalizeNfc
+  else if op = 121uL then Some PrimTextNormalizeNfd
+  else if op = 122uL then Some PrimTextNormalizeNfkc
+  else if op = 123uL then Some PrimTextNormalizeNfkd
+  (* Case mapping: 130-132 *)
+  else if op = 130uL then Some PrimTextToUpper
+  else if op = 131uL then Some PrimTextToLower
+  else if op = 132uL then Some PrimTextToTitle
   else None
